src/proof/controllers/deployment/deployment_init.v
@@ -1,0 +1,24 @@
+From New.proof Require Export fmt.
+From New.proof Require Export prelude.
+From New.proof.k8s_io.api.apps Require Export v1_init.
+From New.proof.k8s_io.api.core Require Export v1_init.
+From New.proof.k8s_io.apimachinery.pkg.api Require Export errors_init.
+From New.proof.k8s_io.apimachinery.pkg.apis.meta Require Export v1_init.
+From New.proof.k8s_io.apimachinery.pkg Require Export labels_init.
+From New.proof.k8s_io.apimachinery.pkg.util Require Export intstr_init.
+From New.proof.k8s_io.kubernetes.pkg Require Export controller_init.
+From New.proof.kubernetes_model Require Export apimodel_init.
+From New.proof Require Export reflect_init.
+Require Export New.generatedproof.controllers.deployment.
+From New.proof Require Import proof_prelude.
+
+
+Section proof.
+Context `{hG: heapGS Σ} `{!ffi_semantics _ _}.
+Context {sem : go.Semantics} {package_sem : deployment.Assumptions}.
+Collection W := sem + package_sem.
+
+#[global] Instance : IsPkgInit (iProp Σ) deployment := define_is_pkg_init True%I.
+#[global] Instance : GetIsPkgInitWf (iProp Σ) deployment := build_get_is_pkg_init_wf.
+
+End proof.
