src/proof/kubernetes_model/apimodel_init.v
@@ -22,6 +22,7 @@ From New.proof.k8s_io.kubernetes.pkg.apis.apps Require Export install_init.
 From New.proof.k8s_io.kubernetes.pkg.apis.apps Require Export v1_init.
 From New.proof.k8s_io.kubernetes.pkg.apis.core Require Export v1_init.
 From New.proof.k8s_io.kubernetes.pkg Require Export controller_init.
+From New.proof.k8s_io.kubernetes.pkg.registry.apps Require Export deployment_init.
 From New.proof.k8s_io.kubernetes.pkg.registry.apps Require Export replicaset_init.
 From New.proof.k8s_io.kubernetes.pkg.registry.apps Require Export statefulset_init.
 From New.proof.k8s_io.kubernetes.pkg.registry.core Require Export pod_init.
